multipleSpecWrites/eraseRollbackIdempotent.v
@@ -20,24 +20,25 @@ Qed.
  
 Inductive actionIDs : thread -> Prop :=
 |nilAct : forall tid s2 M, actionIDs (tid, nil, s2, M)
-|consRead : forall maj min min' tid s1 s2 M N x,
+|consRead : forall maj min min' E tid s1 s2 M N x,
+              decompose N = (E, get (fvar x)) ->
               actionIDs(Tid(maj,min)tid, s1, s2, M) ->
               actionIDs(Tid(maj,min)tid, rAct x (Tid(maj,min') tid) N::s1, s2, M)
-|consWrite : forall maj min min' tid s1 s2 M N x,
+|consWrite : forall maj min min' E tid s1 s2 M N x N',
+               decompose N = (E, put (fvar x) N') ->
                actionIDs(Tid(maj,min)tid, s1, s2, M) ->
                actionIDs(Tid(maj,min)tid, wAct x (Tid(maj,min') tid) N::s1, s2, M)
-|consNew : forall maj min min' tid s1 s2 M N x,
+|consNew : forall maj min min' E tid s1 s2 M N x,
+             decompose N = (E, new) ->
              actionIDs(Tid(maj,min)tid, s1, s2, M) ->
              actionIDs(Tid(maj,min)tid, cAct x (Tid(maj,min') tid) N::s1, s2, M)
 |consSpec : forall maj min min' tid s1 s2 M N,
               actionIDs(Tid(maj,min)tid, s1, s2, M) ->
               actionIDs(Tid(maj,min)tid, sAct (Tid(maj,min') tid) N::s1, s2, M)
-|consFork : forall maj min min' tid s1 s2 M N x,
+|consFork : forall maj min min' tid s1 s2 M N N' E x,
+              decompose N = (E, fork N') -> 
               actionIDs(Tid(maj,min)tid, s1, s2, M) ->
               actionIDs(Tid(maj,min)tid, fAct x (Tid(maj,min') tid) N::s1, s2, M)
-|consJoin : forall maj min tid s1 s2 M,
-              actionIDs(Tid(maj,min)tid, s1, s2, M) ->
-              actionIDs(Tid(maj,min)tid, joinAct::s1, s2, M)
 |consCSpec : forall maj min tid s1 s2 M,
               actionIDs(Tid(maj,min)tid, s1, s2, M) ->
               actionIDs(Tid(maj,min)tid, specAct::s1, s2, M)
@@ -45,113 +46,87 @@ Inductive actionIDs : thread -> Prop :=
 
 Axiom ConsistentIDs : forall T, actionIDs T. 
 
-Inductive actionTerm : action -> trm -> Prop :=
-|readTerm : forall x tid M, actionTerm (rAct x tid M) M
-|writeTerm : forall x tid M, actionTerm (wAct x tid M) M
-|newTerm : forall x tid M, actionTerm (cAct x tid M) M. 
-
-Theorem eraseLastAct : forall tid A s2 M M' T t,
-                         actionTerm A M' ->
-                         eraseThread (tid, [A], s2, M) T t ->
-                         eraseThread (tid, nil, s2, M') T t. 
+Theorem lastActionConsistent : forall tid x a s N,
+                                 actionIDs(tid, x++[a], s, N) -> 
+                                 actionIDs(tid, [a], s, N).
 Proof.
-  intros. inversion H0; subst; try solve[
+  induction x; intros. 
+  {simpl in H. assumption. }
+  {simpl in *. inversion H; subst; auto. }
+Qed. 
+
+Ltac eraseThreadTac :=
   match goal with
-       |H:[?A] = ?s++[?x], H':actionTerm ?A ?M |- _ => 
-        destruct s; inversion H; subst; inversion H'; subst; constructor; auto;
-        invertListNeq
-  end]. 
-  {destruct s1'; inversion H7. subst. inversion H. destruct s1'; inversion H3. }
-  {destruct s1'; inversion H7. subst. inversion H. destruct s1'; inversion H3. }
-Qed. 
+      | |- eraseThread (?tid, [rAct ?x ?tid' ?M], ?s2, ?N) ?T ?m => eapply tEraseRead
+      | |- eraseThread (?tid, [wAct ?x ?tid' ?M], ?s2, ?N) ?T ?m => eapply tEraseWrite
+      | |- eraseThread (?tid, [cAct ?x ?tid' ?M], ?s2, ?N) ?T ?m => eapply tEraseNew
+      | |- eraseThread (?tid, [fAct ?x ?tid' ?M], ?s2, ?N) ?T ?m => eapply tEraseFork
+  end. 
 
-Theorem eraseTwoActs : forall tid A1 A2 As s2 M T t,
-                         eraseThread (tid, (A1::A2::As), s2, M) T t ->
-                         eraseThread (tid, (A2 :: As), s2, M) T t. 
+Theorem eraseLastAct : forall tid tid' A s2 M M' T t,
+                         basicAction A M' tid' ->
+                         (eraseThread (tid, [A], s2, M) T t <->
+                         eraseThread (tid', nil, s2, M') T t). 
 Proof.
-  intros. 
-  inversion H; subst; match goal with
-       |H:?A1::?A2::?As = ?s1 ++ [?x] |- _ => apply listAlign in H;
-                                             invertExists; eauto
-   end. 
-Qed. 
-
-Theorem lookupWeakening : forall tid T t t', thread_lookup T tid t ->
-                                             thread_lookup (tAdd T t') tid t. 
-Proof.
-  intros. inversion H; subst. econstructor. constructor. assumption. reflexivity. 
-Qed. 
-
-Theorem eraseWeaken : forall T t M M', eraseTerm M T M' -> eraseTerm M (tAdd T t) M'.
-Proof.
-  intros. generalize dependent t. induction H; intros; auto. 
-  {econstructor. apply IHeraseTerm1. eassumption. eapply IHeraseTerm2. 
-   eapply lookupWeakening in H2. eassumption. }
-Qed. 
-
-Theorem x : forall T t t' t'' P M M', 
-              eraseThread t P t'' -> eraseThread t' P t'' ->
-              eraseTerm M (tAdd T t) M' ->
-              eraseTerm M (tAdd T t') M'.
-Proof.
-  intros. generalize dependent t'. generalize dependent t''. generalize dependent P. 
-  remember (tAdd T t). induction H1; intros; auto; 
-  try solve[constructor; [eapply IHeraseTerm1; eauto|eauto]];
-  try solve[constructor; eapply IHeraseTerm; eauto].           
-  {econstructor. eapply IHeraseTerm1. assumption. eassumption. assumption. 
-   eassumption. eapply IHeraseTerm2. assumption. eassumption. assumption. 
-   subst. inversion H0; subst. inversion H8; subst; clear H8. inversion H7; subst. 
-   {econstructor. apply Union_introl. eassumption. reflexivity. }
-   {inversion H; subst; clear H. admit. }
+  intros. split; intros. 
+  {inversion H0; subst; try solve[
+            match goal with
+              |H:[?A] = ?s++[?x], H':basicAction ?A ?M ?tid'|- _ => 
+               destruct s; inversion H; subst; inversion H'; subst; constructor; auto;
+               invertListNeq
+            end]. 
+   {destruct s1'; inversion H7. subst. inversion H. destruct s1'; inversion H3. }
+   {destruct s1'; inversion H7. subst. inversion H. destruct s1'; inversion H3. }
+  }
+  {destruct tid. destruct p. destruct tid'. destruct p. inversion H0; subst; try invertListNeq;
+                                                        try solve[
+   inversion H; subst; try solve[ 
+    match goal with
+         | |- eraseThread ?t ?T ?M => assert(C:actionIDs t) by apply ConsistentIDs;
+                                     inversion C; subst
+     end; eraseThreadTac; eauto; rewrite app_nil_l; reflexivity]]; try invertListNeq. 
   }
 Qed. 
 
-Theorem erasePoolSame : forall T T' t t' t'',
-                          erasePool (tAdd T t) T' -> eraseThread t T t'' ->
-                          eraseThread t' T t'' -> erasePool (tAdd T t') T'. 
-Proof.
-  intros. inversion H; subst. 
-  assert(erasePoolAux(tAdd T t) = erasePoolAux(tAdd T t')). 
-  apply Extensionality_Ensembles. unfold Same_set. unfold Included. split; intros. 
-  {inversion H2; subst. inversion H3; subst. inversion H6. 
-   {econstructor. econstructor. econstructor. eassumption. reflexivity. 
-    Focus 2. eassumption. inversion H4; subst. 
-    {econstructor. eapply x. eapply H0. eapply H1. assumption. }
-    {econstructor. reflexivity. eapply x. eapply H0. auto. auto. eassumption. }
-    {eapply tEraseWrite; eauto. eapply x. eapply H0. auto. auto. }
-    {eapply tEraseNew; eauto. eapply x. eapply H0. auto. auto. }
-    {eapply tEraseSpec; eauto. }
-    {eapply tEraseFork; eauto. eapply x. eapply H0; auto. auto. auto. }
-    {eapply tEraseJoin. reflexivity. eapply x. eapply H0. auto. auto. }
-    {eapply tEraseCreatedSpec. reflexivity. }
-   } 
-   (*{inversion H7; subst; clear H7. inversion H8; subst; clear H8.
-    inversion H1; subst. 
-    {destruct tid0. destruct p. econstructor. econstructor. eapply Union_intror. 
-     econstructor. reflexivity. econstructor. eapply x. Focus 2. eapply H1. 
-     econstructor. eassumption. apply eraseWeaken. eassumption. 
 
-  } *)
-Admitted. 
 
-Theorem y : forall T t t' t'' P M M', 
-              eraseThread t P t'' -> eraseThread t' P t'' ->
-              eraseThread M (tAdd T t) M' ->
-              eraseThread M (tAdd T t') M'.
+Hint Resolve app_comm_cons. 
+
+Theorem eraseTwoActs : forall tid tid' A1 A2 As s2 M M' T t,
+                         eraseThread (tid', (A1::A2::As), s2, M') T t <->
+                         eraseThread (tid, (A2 :: As), s2, M) T t. 
 Proof.
-  intros. generalize dependent t'. generalize dependent t''. generalize dependent P. 
-  remember (tAdd T t). induction H1; intros; auto; subst; 
-  try solve[constructor; [eapply IHeraseTerm1; eauto|eauto]];
-  try solve[constructor; eapply IHeraseTerm; eauto].           
-  {constructor. eapply x. eapply H0. assumption. assumption. }
-  {econstructor. reflexivity. eapply x. eapply H2. assumption. assumption. eauto. }
-  {eapply tEraseWrite. reflexivity. eapply x. eapply H2. auto. auto. eauto. }
-  {eapply tEraseNew. reflexivity. eapply x. eapply H2. auto. auto. eauto. }
-  {eapply tEraseSpec. reflexivity. }
-  {eapply tEraseFork. reflexivity. eapply x. eapply H2. auto. auto. eauto. }
-  {eapply tEraseJoin. reflexivity. eapply x. eapply H1. auto. auto. }
-  {eapply tEraseCreatedSpec. reflexivity. }
-Admitted. 
+  intros. split; intros. 
+  {inversion H; subst; match goal with
+       |H:?A1::?A2::?As=?s++[?a] |- _ => apply listAlign in H; invertExists
+        end; match goal with
+               |H:?A::?As=?x++[?a] |- eraseThread(?t,?A::?As,?s2,?m) ?T ?M =>
+                rewrite H; destruct t; destruct p
+             end; match goal with
+                    | |- eraseThread(?t,?s1,?s2,?M) ?T ?M' => assert(C:actionIDs(t, s1, s2, M)) 
+                                                             by apply ConsistentIDs;
+                                                             apply lastActionConsistent in C; 
+                                                             inversion C; subst
+                  end; eauto.
+  }
+  {inversion H; subst; destruct tid'; destruct p;
+   match goal with
+        |H:?A::?As=?s++[?a], H':eraseThread ?t ?T ?M |- eraseThread ?t' ?T ?M'  =>
+         rewrite H; assert(C:actionIDs t') by apply ConsistentIDs; rewrite H in C;
+         rewrite app_comm_cons in C; apply lastActionConsistent in C; inversion C; subst                     
+   end; eauto. 
+  }
+Qed. 
+
+Axiom uniqueThreadPool2 : forall T1 T2 tid t', 
+                            thread_lookup (Union thread T1 T2) tid t' ->
+                            thread_lookup T1 tid t' ->
+                            thread_lookup T2 tid t' -> False. 
+
+Ltac copy H := 
+  match type of H with
+      |?x => assert(x) by assumption
+  end. 
 
 (*Helper theorems for reasoning about the erasure of heaps being rolled back*)
 Theorem eraseHeapRBNew : forall H H' x S A,
@@ -161,7 +136,7 @@ Theorem eraseHeapRBNew : forall H H' x S A,
 Proof.
   induction H; intros. 
   {simpl in H0. inversion H0. }
-  {simpl in *. destruct a. destruct (beq_nat x0 i) eqn:eq. 
+  {simpl in *. destruct a. destruct (beq_nat x i) eqn:eq. 
    {inversion H1; subst; clear H1. inversion H0; subst. assumption. }
    {inversion H0; eauto. }
   }
@@ -174,7 +149,7 @@ Theorem eraseHeapRBRead : forall H H' x sc tid ds S A t N,
 Proof. 
   induction H; intros. 
   {simpl in H0. inversion H0. }
-  {simpl in *. destruct a. destruct (beq_nat x0 i) eqn:eq. 
+  {simpl in *. destruct a. destruct (beq_nat x i) eqn:eq. 
    {inversion H1; subst. clear H1. inversion H0; subst; eauto. 
     apply beq_nat_true in eq. subst. eauto. }
    {inversion H0; eauto. }
@@ -188,7 +163,7 @@ Theorem eraseHeapRBWrite : forall H H' x sc S A tid N,
 Proof.
   induction H; intros. 
   {simpl in H0. inversion H0. }
-  {simpl in *. destruct a. destruct (beq_nat x0 i) eqn:eq. 
+  {simpl in *. destruct a. destruct (beq_nat x i) eqn:eq. 
    {inversion H1; subst. clear H1. inversion H0; subst. 
     econstructor. assumption. apply beq_nat_true in eq. subst. auto. }
    {inversion H0; eauto. }
@@ -199,81 +174,229 @@ Theorem appNil : forall (T:Type) (x:T), [x] = nil ++ [x].
 Proof.
   intros. simpl. reflexivity. Qed. 
 
-Theorem z : forall T t T', erasePool (tAdd T t) T' -> 
-                           exists t', eraseThread t (tAdd T t) t'. 
+Theorem eraseTermDiffPool :  forall tid tid' T t'' P M M' s1 s2 a b N N', 
+              eraseThread (tid', a::b::s1, s2, N') P t'' -> eraseThread (tid, b::s1, s2, N) P t'' ->
+              (eraseTerm M (tAdd T (tid', a::b::s1, s2, N')) M' <->
+              eraseTerm M (tAdd T (tid, b::s1, s2, N)) M'). 
 Proof.
-  Admitted. 
-
-Theorem erasePoolAuxEq : forall A M M' tid tid' s2 T,
-                           actionTerm A M' ->
-                           erasePoolAux(tAdd T (tid, [A], s2, M)) = 
-                           erasePoolAux(tAdd T (tid', nil, s2, M')). 
-Admitted. 
-
-Theorem asdf : forall T t t' t'', 
-                 eraseThread t (tAdd T t) t'' -> eraseThread t' (tAdd T t') t'' ->
-                 erasePoolAux(tAdd T t) = erasePoolAux(tAdd T t'). 
-Proof.
-  intros. apply Extensionality_Ensembles. unfold Same_set. unfold Included. 
-  split; intros. 
-  {inversion H1; subst. inversion H2; subst. inversion H5; subst. 
-   {inversion H6; subst; clear H6. inversion H3; subst. 
-    {inversion H4; subst. clear H4. econstructor. econstructor. apply Union_intror. 
-     
-
-Theorem erasePoolReadEq1 : forall T tid' x0 tid'' M' s2 M,                
-        erasePoolAux(tAdd T (tid',[rAct x0 tid'' M'], s2, M)) = 
-        erasePoolAux(tAdd T (tid'', nil, s2, M')). 
-Proof.
-  intros. apply Extensionality_Ensembles. unfold Same_set. unfold Included. 
-  split; intros. 
-  {inversion H; subst. inversion H0; subst. inversion H3.  
-   {econstructor. econstructor. econstructor; eauto. reflexivity. 
-    Focus 2. eassumption. 
-    assert(exists TE, erasePool(tAdd T (tid',[rAct x0 tid'' M'], s2, M)) TE).
-    exists (erasePoolAux(tAdd T (tid', [rAct x0 tid'' M'], s2, M))). constructor. 
-    invertExists. apply z in H8. invertExists. eapply y. eassumption. 
-    inversion H7; try solve[
-       match goal with
-         |H:?x=?s++[?y]|- _ => destruct s; inversion H; invertListNeq
-       end]. 
-       {destruct s1'; inversion H14; subst. econstructor. assumption. 
-        constructor. invertListNeq. } assumption. } 
-      { destruct tid''. destruct p. inversion H4; subst; clear H4.
-       inversion H5; subst; clear H5. inversion H1; subst; try invertListNeq. 
-       {econstructor. econstructor. apply Union_intror. econstructor. 
-        reflexivity. econstructor.  Focus 2. eassumption. destruct s1'.
-        inversion H12; subst. eapply x. eassumption. econstructor. assumption. 
-        assumption. inversion H12. invertListNeq. }
-      }
-  }
-  {inversion H. inversion H0. inversion H4; subst. 
-   {econstructor. econstructor. econstructor; eauto. reflexivity. 
-    Focus 2. eassumption.
-    assert(exists TE, erasePool(tAdd T (tid',[rAct x0 tid'' M'], s2, M)) TE).
-    exists(erasePoolAux (tAdd T (tid', [rAct x0 tid'' M'], s2, M))). econstructor. 
-    invertExists. apply z in H6. invertExists. eapply y. eassumption. 
-    inversion H3; subst; try solve[
-             match goal with
-               |H:?x=?s++[?y] |- _ => destruct s; inversion H; invertListNeq
-             end]. 
-    {destruct s1'. inversion H13; subst. clear H13. econstructor. rewrite <- appNil. 
-     reflexivity. assumption. eassumption. assumption. }
-    {eapply y. Focus 3. eapply H1. Focus 2. eassumption. inversion H3; subst;
-                                                         try invertListNeq. 
-     {destruct s1'; inversion H13; subst. constructor. assumption. 
-      destruct s1'; inversion H8. }
-    }
+  intros. split; intros. 
+  {remember(tAdd T (tid', a ::b::s1, s2, N')). generalize dependent T. 
+   induction H1; eauto; intros. 
+   {subst. inversion H2; subst. inversion H8; subst; clear H8. inversion H7; subst. 
+    {econstructor. eapply IHeraseTerm1; eauto. reflexivity. eapply IHeraseTerm2; eauto. 
+     econstructor. econstructor. eassumption. reflexivity. }
+    {inversion H1; subst. clear H1. apply listAlign in H5. invertExists.
+     assert(actionIDs(tid, x++[sAct(Tid(maj,min'')tid0)M'], s4, N)). apply ConsistentIDs. 
+     apply lastActionConsistent in H3. inversion H3; subst. econstructor. 
+     eapply IHeraseTerm1. reflexivity. reflexivity. eapply IHeraseTerm2. reflexivity. 
+     econstructor. apply Union_intror. rewrite H1. econstructor. reflexivity. }
    }
-   {destruct tid'. destruct p. inversion H5; subst; clear H5. inversion H9; subst. 
-    clear H9. inversion H1; subst; try invertListNeq. 
-    {econstructor. econstructor. apply Union_intror. econstructor. reflexivity.
-     
+  }
+  {remember(tAdd T (tid, b :: s1, s2, N)). generalize dependent T. induction H1; auto. 
+   {intros. subst. inversion H2; subst. inversion H7; subst. 
+    {inversion H8; subst; clear H8. econstructor. eapply IHeraseTerm1; eauto. 
+     reflexivity. eapply IHeraseTerm2; eauto. econstructor. econstructor. eauto. eauto. }
+    {inversion H8; subst; clear H8. inversion H1; subst; clear H1. 
+     assert(actionIDs(tid', a::s1'++[sAct(Tid(maj,min'')tid0)M'], s4, N')). apply ConsistentIDs. 
+     rewrite app_comm_cons in H1. apply lastActionConsistent in H1. inversion H1; subst. 
+     econstructor. eapply IHeraseTerm1; eauto. reflexivity. eapply IHeraseTerm2; eauto. 
+     econstructor. apply Union_intror. rewrite H5. rewrite app_comm_cons. econstructor. 
+     reflexivity. }
+   }
+  }
+Qed. 
 
+Theorem eraseThreadDiffPool : forall tid tid' T t'' P M M' s1 s2 a b N N', 
+              eraseThread (tid', a::b::s1, s2, N') P t'' -> eraseThread (tid, b::s1, s2, N) P t'' ->
+              (eraseThread M (tAdd T (tid', a::b::s1, s2, N')) M' <->
+              eraseThread M (tAdd T (tid, b::s1, s2, N)) M'). 
+Proof.
+  intros. split; intros. 
+  {inversion H1. 
+   {constructor. subst. eapply eraseTermDiffPool; eauto. }
+   {subst. eapply tEraseRead. reflexivity. eapply eraseTermDiffPool; eauto. eassumption. }
+   {subst. eapply tEraseWrite. reflexivity. eapply eraseTermDiffPool; eauto. eassumption. }
+   {subst. eapply tEraseNew. reflexivity. eapply eraseTermDiffPool; eauto. eauto. }
+   {subst. eapply tEraseSpec. reflexivity. }
+   {subst. eapply tEraseFork. reflexivity. eapply eraseTermDiffPool; eauto. eauto. }
+   {subst. eapply tEraseCreatedSpec. reflexivity. }
+  }
+  {inversion H1; subst; eauto. 
+   {econstructor. eapply eraseTermDiffPool; eauto. }
+   {econstructor. reflexivity. eapply eraseTermDiffPool; eauto. eauto. }
+   {eapply tEraseWrite; eauto. eapply eraseTermDiffPool; eauto. }
+   {eapply tEraseNew; eauto. eapply eraseTermDiffPool; eauto. }
+   {eapply tEraseFork; eauto. eapply eraseTermDiffPool; eauto. }
+  }
+Qed. 
 
-     Admitted.
+Theorem eraseTermStrengthen : forall s1 s2 t t' T tid a M, 
+              (forall tid' M', a <> sAct tid' M') ->
+              eraseTerm t (tAdd T (tid, s1++[a], s2, M)) t' ->
+              eraseTerm t T t'.
+Proof.
+  intros. remember (tAdd T (tid, s1 ++ [a], s2, M)). induction H0; auto. 
+  {subst. inversion H1; subst. inversion H7; subst. clear H7. inversion H6; subst. 
+   {econstructor. eapply IHeraseTerm1; eauto. reflexivity. eapply IHeraseTerm2. reflexivity. 
+    econstructor. eassumption. reflexivity. }
+   {inversion H0; subst. apply lastElementEq in H4. unfold not in H. apply H in H4. inversion H4. }
+  }
+Qed. 
 
+Theorem eraseTermStrengthenNil : forall t t' T tid s2 M,
+                                   eraseTerm t (tAdd T (tid, nil, s2, M)) t' ->
+                                   eraseTerm t T t'. 
+Proof.
+  intros. remember (tAdd T (tid, nil, s2, M)). induction H; auto. 
+  {subst. inversion H2; subst. inversion H7; subst. 
+   {econstructor. apply IHeraseTerm1. reflexivity. reflexivity. eapply IHeraseTerm2. 
+    reflexivity. econstructor. eassumption. reflexivity. }
+   {inversion H0; subst. invertListNeq. }
+  }
+Qed. 
 
+Theorem eraseTermWeakening : forall t t' T T', 
+                                 eraseTerm t T t' ->
+                                 eraseTerm t (tAdd T T') t'.  
+Proof.
+  intros. induction H; eauto. 
+  {inversion H2; subst. econstructor. eapply IHeraseTerm1. reflexivity. eapply IHeraseTerm2. 
+   econstructor. econstructor. inversion H2. eassumption. reflexivity. }
+Qed. 
+
+Theorem eraseThreadStrengthenNil : forall t t' tid' T s2 M,
+                                     eraseThread t (tAdd T (tid', nil, s2, M)) t' ->
+                                     eraseThread t T t'.
+Proof.
+  intros. inversion H; subst. 
+  {econstructor. eapply eraseTermStrengthenNil. eauto. }
+  {econstructor. reflexivity. eapply eraseTermStrengthenNil. eauto. eauto. }
+  {eapply tEraseWrite. reflexivity. eapply eraseTermStrengthenNil. eauto. eauto. }
+  {eapply tEraseNew. reflexivity. eapply eraseTermStrengthenNil. eauto. eauto. }
+  {eapply tEraseSpec. reflexivity. }
+  {eapply tEraseFork. reflexivity. eapply eraseTermStrengthenNil. eauto. eauto. }
+  {eapply tEraseCreatedSpec. reflexivity. }
+Qed. 
+
+Theorem eraseThreadStrengthen : forall t t' T tid' a s1 s2 M, 
+              (forall tid M', a <> sAct tid M') ->
+              eraseThread t (tAdd T (tid', s1 ++ [a], s2, M)) t' ->
+              eraseThread t T t'. 
+Proof.
+  intros. inversion H0; subst; try solve[match goal with
+       |H:eraseTerm ?M ?T ?M' |- _ => eapply eraseTermStrengthen in H; eauto
+   end]. 
+  {econstructor. reflexivity. }
+  {econstructor. reflexivity. }
+Qed. 
+
+Theorem eraseThreadWeakening : forall t t' T T', 
+                                 eraseThread t T t' ->
+                                 eraseThread t (tAdd T T') t'. 
+Proof.
+  intros. inversion H; subst. 
+  {econstructor. apply eraseTermWeakening. assumption. }
+  {econstructor. reflexivity. apply eraseTermWeakening; eauto. eassumption. }
+  {eapply tEraseWrite. reflexivity. apply eraseTermWeakening; eauto. eassumption. }
+  {eapply tEraseNew; eauto. apply eraseTermWeakening; eauto. }
+  {eapply tEraseSpec; eauto. }
+  {eapply tEraseFork; eauto. apply eraseTermWeakening; eauto. }
+  {eapply tEraseCreatedSpec; eauto. }
+Qed. 
+
+Theorem eraseExists : forall T t T', 
+                        erasePool (tAdd T t) T' -> exists t', eraseThread t (tAdd T t) t'. 
+Proof.
+  intros. eapply erasePoolEraseThread. eassumption. apply Union_intror. constructor. Qed. 
+
+Theorem eraseBasicAction2 : forall a b s1' s2 M M' tid tid' T,
+                              basicAction a M' tid' ->
+                              erasePoolAux(tAdd T (tid, a::b::s1', s2, M)) = 
+                              erasePoolAux(tAdd T (tid', b::s1', s2, M')). 
+Proof.
+  intros. apply Extensionality_Ensembles. unfold Same_set. unfold Included. split; intros. 
+  {inversion H0; subst. inversion H1; subst. inversion H5; subst; clear H5. inversion H4; subst. 
+   {econstructor. econstructor. econstructor. eassumption. reflexivity. 
+    assert(exists y, erasePool (tAdd T (tid, a::b::s1', s2, M)) y). eauto. invertExists. 
+    apply eraseExists in H7. invertExists. eapply eraseThreadDiffPool. Focus 3. 
+    eassumption. eassumption. eapply eraseTwoActs. eassumption. assumption. }
+   {destruct tid'. destruct p. econstructor. econstructor. apply Union_intror. econstructor. 
+    reflexivity. Focus 2. eassumption. inversion H5; subst; clear H5. inversion H; subst;
+     try solve[match goal with
+       |H:eraseThread ?t ?T ?M |- eraseThread(?tid, ?s1,?s2,?Masd') ?T' ?N => 
+        assert(C:actionIDs t) by apply ConsistentIDs; inversion C; subst
+     end; copy H2; apply eraseTwoActs with(tid0:= Tid(n,n0) l) (M:=M')in H2; 
+                       eapply eraseThreadDiffPool; eauto]. 
+   }
+  }
+  {inversion H0; subst. inversion H1; subst. inversion H5; subst; clear H5. inversion H4; subst. 
+   {econstructor. econstructor. econstructor. eassumption. reflexivity. 
+    assert(exists y, erasePool(tAdd T (tid', b :: s1', s2, M')) y); eauto. invertExists. 
+    apply eraseExists in H7. invertExists. eapply eraseThreadDiffPool. eapply eraseTwoActs. 
+    eassumption. eassumption. eassumption. assumption. }
+   {destruct tid. destruct p. econstructor. econstructor. apply Union_intror. econstructor. 
+    reflexivity. inversion H5; subst; clear H5. inversion H; subst; try solve[ 
+     match goal with
+         |H:eraseThread ?t ?T ?M |- eraseThread (?tid,?s1,?s2,?N) ?T' ?M' =>
+          assert(C:actionIDs (tid,s1,s2,N)) by apply ConsistentIDs; inversion C; subst
+     end; eapply eraseTwoActs; eapply eraseThreadDiffPool; [eapply eraseTwoActs; eauto|eauto|eauto]]. 
+    assumption. }
+  }
+Qed. 
+
+Theorem erasePoolCSpec : forall T tid s2 N l,
+                           erasePoolAux(tAdd T (tid, l++[specAct], s2, N)) = erasePoolAux T. 
+Proof.
+  intros. apply Extensionality_Ensembles. unfold Same_set. unfold Included. split; intros.  
+  {inversion H; subst. inversion H0; subst. inversion H4; subst; clear H4. inversion H3; subst. 
+   {econstructor. econstructor. eassumption. reflexivity. 
+    apply eraseThreadStrengthen in H1. eassumption. intros. intros c. inversion c. auto. }
+   {inversion H4; subst; clear H4. inversion H1; try invertListNeq. 
+    {subst. inversion H2. }
+   }
+  }
+  {inversion H; subst. inversion H0; subst. inversion H4; subst; clear H4. econstructor. 
+   econstructor. econstructor. eassumption. reflexivity. eapply eraseThreadWeakening.
+   eassumption. eassumption. }
+Qed. 
+  
+Theorem eraseBasicAction1 : forall a M M' s2 tid tid' T,
+                               basicAction a M' tid' ->
+                               erasePoolAux(tAdd T (tid, [a], s2, M)) = 
+                               erasePoolAux(tAdd T (tid', nil, s2, M')). 
+Proof.
+  intros. apply Extensionality_Ensembles. unfold Same_set. unfold Included. split; intros. 
+  {inversion H0; subst. inversion H1; subst. inversion H5; subst; clear H5. inversion H4; subst. 
+   {econstructor. econstructor. econstructor. eassumption. reflexivity. 
+    rewrite appNil in H2. eapply eraseThreadStrengthen in H2. apply eraseThreadWeakening. 
+    eassumption. intros. intros c. inversion H; subst; inversion H6. assumption. }
+   {destruct tid'. destruct p. econstructor. econstructor. eapply Union_intror. econstructor. 
+    reflexivity. inversion H5; subst; clear H5. inversion H; subst; try solve[
+    match goal with
+         |H:eraseThread ?t ?T ?t' |- _ => assert(C:actionIDs t) by apply ConsistentIDs;
+                                         inversion C; subst; eapply eraseLastAct; eauto;
+                                         rewrite appNil in H; eapply eraseThreadStrengthen in H;
+                                         [idtac|intros;intros c; inversion c]; eapply eraseThreadWeakening;
+                                         eauto
+                                         
+                                         
+     end]. 
+    auto. }
+  }
+  {inversion H0; subst. inversion H1; subst. inversion H5; subst; clear H5. inversion H4; subst. 
+   {econstructor. econstructor. econstructor. eassumption. reflexivity. 
+    apply eraseThreadStrengthenNil in H2. eapply eraseThreadWeakening. eassumption. assumption. }
+   {destruct tid. destruct p. econstructor. econstructor. apply Union_intror. econstructor. 
+    reflexivity. inversion H5; subst; clear H5. inversion H; subst; try solve[
+    match goal with
+         |H:eraseThread ?t ?T ?m |- eraseThread ?t' ?T' ?m' =>
+          assert(C:actionIDs t') by apply ConsistentIDs; inversion C; subst;
+          eapply eraseLastAct; [econstructor|idtac]; apply eraseThreadStrengthenNil in H;
+          apply eraseThreadWeakening; eauto
+     end]. assumption. }
+  }
+Qed. 
+  
 Theorem rollbackIdempotent : forall tid stack H T H' T' H'' T'', 
                                rollback tid stack H T H' T' -> 
                                eraseHeap H H'' -> erasePool T T'' ->
@@ -283,70 +406,35 @@ Proof.
   induction H0; intros; subst. {split; auto. }
   {destruct s1'. 
    {eapply IHrollback. inversion H5; subst. 
-    assert(erasePoolAux(tAdd T (tid',[rAct x0 tid'' M'], s2, M)) = 
-           erasePoolAux(tAdd T (tid'', nil, s2, M'))). 
-    {apply Extensionality_Ensembles. unfold Same_set. unfold Included. 
-     split; intros.  
-     {inversion H; subst. inversion H1; subst. inversion H8. 
-      {econstructor. econstructor. econstructor; eauto. reflexivity. 
-       Focus 2. eassumption. apply z in H5. invertExists. eapply y. eassumption. 
-       rewrite appNil in H12. inversion H12; try solve[
-       match goal with
-         |H:?x=?s++[?y]|- _ => destruct s; inversion H; invertListNeq
-       end]. 
-       {destruct s1'; inversion H18; subst. econstructor. assumption. 
-        constructor. invertListNeq. } assumption. } 
-      {destruct tid''. destruct p. inversion H10; subst. clear H10. 
-       inversion H3; subst; try invertListNeq.
-       {econstructor. econstructor. eapply Union_intror. econstructor. 
-        reflexivity. econstructor. Focus 2. eassumption. destruct s1'. 
-        inversion H18; subst. eapply x. eapply H3. econstructor. 
-        assumption. assumption. inversion H18. invertListNeq. }
-      }
-     }
-     {inversion H; subst. inversion H1; subst. inversion H8; subst. 
-      {econstructor. econstructor. econstructor; eauto. reflexivity. 
-       Focus 2. eassumption. apply z in H5. invertExists. eapply y. eassumption.
-       assumption. inversion H9; subst; clear H9. inversion H3; subst. 
-       {inversion H11; subst. 
-        {destruct s1'. inversion H17; subst. clear H17. econstructor. 
-         eapply x. Focus 2. eapply H11. eassumption. eassumption. 
-
-
-
-econstructor. eapply x. Focus 2. eapply H11. eassumption. eassumption.   
-        assert(actionIDs (tid', [rAct x0 tid'' M'], s2, M)). apply ConsistentIDs. 
-        inversion H5; subst. econstructor. rewrite <- appNil. reflexivity.
-
-
-
-       inversion H11; subst; try solve[
-       match goal with
-           |H:?x=?s++[?y] |- _ => destruct s; inversion H; invertListNeq
-       end]. 
-       {inversion H9; subst; clear H9. destruct s1'. inversion H17; subst. econstructor; eauto. auto. }
-       {
-
-admit. }
-    }
-    rewrite H. constructor. eapply eraseHeapRBRead; eauto. }
-   {eapply IHrollback. admit. eapply eraseHeapRBRead; eauto. }
+    erewrite eraseBasicAction1. econstructor. econstructor. eapply eraseHeapRBRead; eauto. }
+   {eapply IHrollback. inversion H5; subst. erewrite eraseBasicAction2. econstructor. 
+    constructor. eapply eraseHeapRBRead; eauto. }
   }
   {destruct s1'. 
-   {eapply IHrollback. admit. assumption. }
-   {eapply IHrollback. admit. assumption. }
+   {eapply IHrollback. inversion H5; subst. rewrite appNil with (x:=specAct). rewrite erasePoolCSpec. 
+    erewrite eraseBasicAction1. econstructor. constructor. assumption. }
+   {eapply IHrollback. inversion H5; subst. rewrite appNil. rewrite erasePoolCSpec. 
+    erewrite eraseBasicAction2; eauto. constructor. assumption. }
   }
   {destruct s1'. 
-   {eapply IHrollback. admit. eapply eraseHeapRBWrite; eauto. }
-   {eapply IHrollback. admit. eapply eraseHeapRBWrite; eauto. }
+   {eapply IHrollback. inversion H5; subst. erewrite eraseBasicAction1. 
+    econstructor. constructor. eapply eraseHeapRBWrite; eauto. }
+   {eapply IHrollback. inversion H5; subst. erewrite eraseBasicAction2; eauto. 
+    constructor. eapply eraseHeapRBWrite; eauto. }
   }
   {destruct s1'. 
-   {eapply IHrollback. admit. eapply eraseHeapRBNew; eauto. }
-   {eapply IHrollback. admit. eapply eraseHeapRBNew; eauto. }
+   {eapply IHrollback. inversion H5; subst. erewrite eraseBasicAction1. 
+    econstructor. constructor. eapply eraseHeapRBNew; eauto. }
+   {eapply IHrollback. inversion H5; subst. erewrite eraseBasicAction2; eauto. 
+    constructor. eapply eraseHeapRBNew; eauto. }
   }
   {destruct s1'. 
-   {eapply IHrollback. admit. assumption. }
-   {eapply IHrollback. admit. assumption. }
+   {eapply IHrollback. inversion H5; subst. 
+    replace [sAct tid2 N'; specAct] with ([sAct tid2 N']++[specAct]). rewrite erasePoolCSpec. 
+    erewrite eraseBasicAction1. econstructor. constructor. auto. assumption. }
+   {eapply IHrollback. inversion H5; subst. 
+    replace [sAct tid2 N';specAct] with ([sAct tid2 N']++[specAct]). rewrite erasePoolCSpec. 
+    erewrite eraseBasicAction2. econstructor. constructor. auto. assumption. }
   }
 Qed. 
 
